txn-data-consistency/EP+_TCCv_invariants.thy
@@ -16,16 +16,9 @@ subsection \<open>Helper functions lemmas: arg_max, add_to_readerset, pending_wt
 lemma view_of_prefix:
   assumes "\<And>k. prefix (corder k) (corder' k)"
     and "\<And>k. distinct (corder' k)"
-    and "\<And>k. u `` {k} \<subseteq> set (corder k)"
+    and "\<And>k. (set (corder' k) - set (corder k)) \<inter> u = {}"
   shows "view_of corder u = view_of corder' u" oops
 
-lemma get_ctx_step:
-  assumes "cl_state (cls s cl) = RtxnInProg keys kvt_map"
-    and "kvt_map k = None"
-    and "cl_state (cls s' cl) = RtxnInProg keys (kvt_map (k \<mapsto> (v, t)))"
-    and "svr_state (svrs s k) t = Commit cts v rs deps"
-    and "\<And>k t. svr_state (svrs s' k) t = svr_state (svrs s k) t"
-  shows "get_ctx s' (kvt_map (k \<mapsto> (v, t))) = get_ctx s kvt_map \<union> (insert (k, t) deps)" oops
 
 subsection \<open>Extra: general lemmas: find, min, append\<close>
 
@@ -74,18 +67,18 @@ lemma lst_map_monotonic:
 
 definition Finite_Dom_Kv_map where
   "Finite_Dom_Kv_map s cl \<longleftrightarrow>
-    (\<forall>kv_map cts deps. cl_state (cls s cl) \<in> {WtxnPrep kv_map, WtxnCommit cts kv_map deps} \<longrightarrow>
+    (\<forall>kv_map cts. cl_state (cls s cl) \<in> {WtxnPrep kv_map, WtxnCommit cts kv_map} \<longrightarrow>
       finite (dom (kv_map)))"
 
-definition Finite_Dom_Kvt_map where
-  "Finite_Dom_Kvt_map s cl \<longleftrightarrow>
-    (\<forall>keys kvt_map. cl_state (cls s cl) = RtxnInProg keys kvt_map \<longrightarrow>
-      finite (dom (kvt_map)) \<and> keys \<noteq> {})"
+definition Finite_Dom_Kv_map_rd where
+  "Finite_Dom_Kv_map_rd s cl \<longleftrightarrow>
+    (\<forall>keys kv_map. cl_state (cls s cl) = RtxnInProg keys kv_map \<longrightarrow>
+      finite (dom (kv_map)) \<and> keys \<noteq> {})"
 
 definition Finite_t_Ran_Kvt_map where
   "Finite_t_Ran_Kvt_map s cl \<longleftrightarrow>
-    (\<forall>keys kvt_map. cl_state (cls s cl) = RtxnInProg keys kvt_map \<longrightarrow>
-      finite (snd ` ran (kvt_map)))"
+    (\<forall>keys kv_map. cl_state (cls s cl) = RtxnInProg keys kv_map \<longrightarrow>
+      finite (snd ` ran (kv_map)))"
 
 definition Finite_Lst_map_Ran where
   "Finite_Lst_map_Ran s cl \<longleftrightarrow> finite (range (lst_map (cls s cl)))"
@@ -134,7 +127,7 @@ definition KvsOfS_Not_Emp where
   "KvsOfS_Not_Emp s \<longleftrightarrow> (\<forall>k. kvs_of_s s k \<noteq> [])"
 
 definition Init_Ver_Inv where
-  "Init_Ver_Inv s k \<longleftrightarrow> (\<exists>rs. svr_state (svrs s k) T0 = Commit 0 undefined rs {})"
+  "Init_Ver_Inv s k \<longleftrightarrow> (\<exists>rs. svr_state (svrs s k) T0 = Commit 0 undefined rs)"
 
 
 subsection \<open>Invariant about server and client state relations and (future and past) transactions ids\<close>
@@ -154,7 +147,7 @@ definition Cl_Rtxn_Inv where
 
 definition Cl_Wtxn_Idle_Svr where
   "Cl_Wtxn_Idle_Svr s \<longleftrightarrow>
-    (\<forall>cl k cts kv_map deps. cl_state (cls s cl) \<in> {WtxnPrep kv_map, WtxnCommit cts kv_map deps}
+    (\<forall>cl k cts kv_map. cl_state (cls s cl) \<in> {WtxnPrep kv_map, WtxnCommit cts kv_map}
         \<and> kv_map k = None \<longrightarrow> svr_state (svrs s k) (get_wtxn s cl) = No_Ver)"
 
 definition Cl_Prep_Inv where
@@ -163,9 +156,10 @@ definition Cl_Prep_Inv where
     (k \<notin> dom kvm \<longrightarrow> svr_state (svrs s k) (get_wtxn s cl) = No_Ver))"
 
 definition Cl_Commit_Inv where
-  "Cl_Commit_Inv s \<longleftrightarrow> (\<forall>cl k cts kvm deps. \<exists>prep_t v rs. cl_state (cls s cl) = WtxnCommit cts kvm deps
-    \<longrightarrow> (k \<in> dom kvm \<longrightarrow> svr_state (svrs s k) (get_wtxn s cl) \<in> {Prep prep_t v, Commit cts v rs deps}) \<and>
-    (kvm k = None \<longrightarrow> svr_state (svrs s k) (get_wtxn s cl) = No_Ver))"
+  "Cl_Commit_Inv s \<longleftrightarrow> (\<forall>cl k cts kv_map. cl_state (cls s cl) = WtxnCommit cts kv_map \<longrightarrow>
+    (\<forall>v. kv_map k = Some v \<longrightarrow>
+      (\<exists>prep_t rs. svr_state (svrs s k) (get_wtxn s cl) \<in> {Prep prep_t v, Commit cts v rs})) \<and>
+    (kv_map k = None \<longrightarrow> svr_state (svrs s k) (get_wtxn s cl) = No_Ver))"
 
 \<comment> \<open>Next 2 invariants: svr_state \<longrightarrow> cl_state\<close>
 definition Prep_is_Curr_wt where
@@ -173,26 +167,26 @@ definition Prep_is_Curr_wt where
 
 definition Svr_Prep_Inv where
   "Svr_Prep_Inv s \<longleftrightarrow> (\<forall>k t ts v. svr_state (svrs s k) t = Prep ts v \<longrightarrow>
-    (\<exists>cts kv_map deps.
-      cl_state (cls s (get_cl_w t)) \<in> {WtxnPrep  kv_map, WtxnCommit cts kv_map deps} \<and>
+    (\<exists>cts kv_map.
+      cl_state (cls s (get_cl_w t)) \<in> {WtxnPrep  kv_map, WtxnCommit cts kv_map} \<and>
       k \<in> dom kv_map))"
 
 definition Svr_Commit_Inv where
-  "Svr_Commit_Inv s \<longleftrightarrow> (\<forall>k t cts v rs deps. 
-    svr_state (svrs s k) t = Commit cts v rs deps \<and> is_curr_wt s t \<longrightarrow> 
-      (\<exists>kv_map. cl_state (cls s (get_cl_w t)) = WtxnCommit cts kv_map deps \<and> k \<in> dom kv_map))"
+  "Svr_Commit_Inv s \<longleftrightarrow> (\<forall>k t cts v rs. 
+    svr_state (svrs s k) t = Commit cts v rs \<and> is_curr_wt s t \<longrightarrow> 
+      (\<exists>kv_map. cl_state (cls s (get_cl_w t)) = WtxnCommit cts kv_map \<and> k \<in> dom kv_map))"
 
 \<comment> \<open>Values of svr_state and rtxn_rts for past transaction ids\<close>
 definition PTid_Inv where
   "PTid_Inv s cl \<longleftrightarrow> (\<forall>k. \<forall>n < cl_sn (cls s cl).
    (svr_state (svrs s k) (Tn (Tn_cl n cl)) = No_Ver) \<or>
    (rtxn_rts s (Tn_cl n cl) = None \<and> 
-    (\<exists>cts v rs deps. svr_state (svrs s k) (Tn (Tn_cl n cl)) = Commit cts v rs deps)))"
+    (\<exists>cts v rs. svr_state (svrs s k) (Tn (Tn_cl n cl)) = Commit cts v rs)))"
 
 lemma other_sn_idle:  
   assumes "FTid_Wtxn_Inv s cl" and "PTid_Inv s cl"
     and "get_cl t = cl" and "get_sn t \<noteq> cl_sn (cls s cl)"
-  shows "\<And>k. \<exists>cts v rs deps. svr_state (svrs s k) (Tn t) \<in> {No_Ver, Commit cts v rs deps}" oops
+  shows "\<And>k. \<exists>cts v rs. svr_state (svrs s k) (Tn t) \<in> {No_Ver, Commit cts v rs}" oops
 
 definition Rtxn_Wtxn_No_Ver where
   "Rtxn_Wtxn_No_Ver s cl \<longleftrightarrow>
@@ -200,30 +194,30 @@ definition Rtxn_Wtxn_No_Ver where
 
 definition Wtxn_Rtxn_None where
   "Wtxn_Rtxn_None s k \<longleftrightarrow>
-    (\<forall>cl n ts v cts rs deps. svr_state (svrs s k) (Tn (Tn_cl n cl)) \<in> {Prep ts v, Commit cts v rs deps}
+    (\<forall>cl n ts v cts rs. svr_state (svrs s k) (Tn (Tn_cl n cl)) \<in> {Prep ts v, Commit cts v rs}
        \<longrightarrow> rtxn_rts s (Tn_cl n cl) = None)"
 
 definition WtxnCommit_Wtxn_Cts where
-  "WtxnCommit_Wtxn_Cts s cl \<longleftrightarrow> (\<forall>cts kv_map deps. cl_state (cls s cl) = WtxnCommit cts kv_map deps
+  "WtxnCommit_Wtxn_Cts s cl \<longleftrightarrow> (\<forall>cts kv_map. cl_state (cls s cl) = WtxnCommit cts kv_map
     \<longrightarrow> wtxn_cts s (get_wtxn s cl) = Some cts)"
 
 definition Wtxn_State_Cts where
-  "Wtxn_State_Cts s k \<longleftrightarrow> (\<forall>t cts v rs deps ts kv_map.
-    svr_state (svrs s k) t = Commit cts v rs deps \<or>
-   (svr_state (svrs s k) t = Prep ts v \<and> cl_state (cls s (get_cl_w t)) = WtxnCommit cts kv_map deps)
+  "Wtxn_State_Cts s k \<longleftrightarrow> (\<forall>t cts v rs ts kv_map.
+    svr_state (svrs s k) t = Commit cts v rs \<or>
+   (svr_state (svrs s k) t = Prep ts v \<and> cl_state (cls s (get_cl_w t)) = WtxnCommit cts kv_map)
       \<longrightarrow> wtxn_cts s t = Some cts)"
 
 definition FTid_notin_rs where
-  "FTid_notin_rs s cl \<longleftrightarrow> (\<forall>k n t cts v rs deps. n > cl_sn (cls s cl) \<and>
-    svr_state (svrs s k) t = Commit cts v rs deps \<longrightarrow> Tn_cl n cl \<notin> rs)"
+  "FTid_notin_rs s cl \<longleftrightarrow> (\<forall>k n t cts v rs. n > cl_sn (cls s cl) \<and>
+    svr_state (svrs s k) t = Commit cts v rs \<longrightarrow> Tn_cl n cl \<notin> rs)"
 
 definition FTid_not_wr where
   "FTid_not_wr s cl \<longleftrightarrow> (\<forall>n k. n > cl_sn (cls s cl) \<longrightarrow> Tn (Tn_cl n cl) \<notin> wtxns_dom (svr_state (svrs s k)))"
 
 definition Fresh_wr_notin_rs where
-  "Fresh_wr_notin_rs s cl \<longleftrightarrow> (\<forall>k t cts kv_map deps cts' v' rs' deps'.
-    cl_state (cls s cl) \<in> {Idle, WtxnPrep kv_map, WtxnCommit cts kv_map deps} \<and>
-    svr_state (svrs s k) t = Commit cts' v' rs' deps' \<longrightarrow> get_txn s cl \<notin> rs')"
+  "Fresh_wr_notin_rs s cl \<longleftrightarrow> (\<forall>k t cts kv_map cts' v' rs'.
+    cl_state (cls s cl) \<in> {Idle, WtxnPrep kv_map, WtxnCommit cts kv_map} \<and>
+    svr_state (svrs s k) t = Commit cts' v' rs' \<longrightarrow> get_txn s cl \<notin> rs')"
 
 definition Fresh_wr_notin_Wts_dom where
   "Fresh_wr_notin_Wts_dom s cl \<longleftrightarrow> (\<forall>keys kv_map k. cl_state (cls s cl) \<in> {Idle, RtxnInProg keys kv_map} \<longrightarrow>
@@ -239,11 +233,11 @@ definition Gst_le_Pts where
       svr_state (svrs s k) (get_wtxn s cl) = Prep prep_t v \<longrightarrow> gst (cls s cl) \<le> prep_t)"
 
 definition Gst_Lt_Cts where
-  "Gst_Lt_Cts s cl \<longleftrightarrow> (\<forall>k cts v rs deps. 
-      svr_state (svrs s k) (get_wtxn s cl) = Commit cts v rs deps \<longrightarrow> gst (cls s cl) < cts)" (*RInvoke & CommitW*)
+  "Gst_Lt_Cts s cl \<longleftrightarrow> (\<forall>k cts v rs. 
+      svr_state (svrs s k) (get_wtxn s cl) = Commit cts v rs \<longrightarrow> gst (cls s cl) < cts)" (*RInvoke & CommitW*)
 
 definition Gst_Lt_Cl_Cts where
-  "Gst_Lt_Cl_Cts s cl \<longleftrightarrow> (\<forall>cl' cts kv_map deps. cl_state (cls s cl') = WtxnCommit cts kv_map deps
+  "Gst_Lt_Cl_Cts s cl \<longleftrightarrow> (\<forall>cl' cts kv_map. cl_state (cls s cl') = WtxnCommit cts kv_map
     \<longrightarrow> gst (cls s cl) < cts)" (*RInvoke & CommitW*)
 
 
@@ -253,11 +247,11 @@ abbreviation is_committed_in_kvs where
   "is_committed_in_kvs s k t \<equiv> 
     is_committed (svr_state (svrs s k) t)  \<or> 
     (is_prepared (svr_state (svrs s k) t) \<and> \<comment> \<open>is_curr_wt s t \<and>\<close>
-     (\<exists>cts kv_map deps. cl_state (cls s (get_cl_w t)) = WtxnCommit cts kv_map deps))"
+     (\<exists>cts kv_map. cl_state (cls s (get_cl_w t)) = WtxnCommit cts kv_map))"
 
 definition CO_Tid where
   "CO_Tid s cl \<longleftrightarrow> (case cl_state (cls s cl) of
-    WtxnCommit cts kv_map deps \<Rightarrow> (\<forall>k n. Tn (Tn_cl n cl) \<in> set (commit_order s k) \<longrightarrow> n \<le> cl_sn (cls s cl))
+    WtxnCommit cts kv_map \<Rightarrow> (\<forall>k n. Tn (Tn_cl n cl) \<in> set (commit_order s k) \<longrightarrow> n \<le> cl_sn (cls s cl))
   | _ \<Rightarrow> (\<forall>k n. Tn (Tn_cl n cl) \<in> set (commit_order s k) \<longrightarrow> n < cl_sn (cls s cl)))"
 
 definition CO_Distinct where
@@ -265,16 +259,16 @@ definition CO_Distinct where
 
 definition CO_Tn_is_Cmt_Abs where
   "CO_Tn_is_Cmt_Abs s k \<longleftrightarrow> (\<forall>n cl. Tn (Tn_cl n cl) \<in> set (commit_order s k) \<longrightarrow>
-    (\<exists>cts v rs deps. svr_state (svrs s k) (Tn (Tn_cl n cl)) = Commit cts v rs deps) \<or> 
+    (\<exists>cts v rs. svr_state (svrs s k) (Tn (Tn_cl n cl)) = Commit cts v rs) \<or> 
     ((\<exists>ts v. svr_state (svrs s k) (Tn (Tn_cl n cl)) = Prep ts v) \<and> 
-     (\<exists>cts kv_map deps. cl_state (cls s cl) = WtxnCommit cts kv_map deps \<and> 
+     (\<exists>cts kv_map. cl_state (cls s cl) = WtxnCommit cts kv_map \<and> 
       cl_sn (cls s cl) = n \<and> k \<in> dom kv_map)))"
 
 definition CO_is_Cmt_Abs where
   "CO_is_Cmt_Abs s k \<longleftrightarrow> (\<forall>t. t \<in> set (commit_order s k) \<longrightarrow>
-    (\<exists>cts v rs deps. svr_state (svrs s k) t = Commit cts v rs deps) \<or> 
+    (\<exists>cts v rs. svr_state (svrs s k) t = Commit cts v rs) \<or> 
     ((\<exists>ts v. svr_state (svrs s k) t = Prep ts v) \<and> 
-     (\<exists>cts kv_map deps. cl_state (cls s (get_cl_w t)) = WtxnCommit cts kv_map deps \<and> k \<in> dom kv_map)))"
+     (\<exists>cts kv_map. cl_state (cls s (get_cl_w t)) = WtxnCommit cts kv_map \<and> k \<in> dom kv_map)))"
 
 definition CO_not_No_Ver where
   "CO_not_No_Ver s k \<longleftrightarrow> (\<forall>t \<in> set (commit_order s k). svr_state (svrs s k) t \<noteq> No_Ver)"
@@ -284,16 +278,16 @@ definition CO_has_Cts where
 
 definition Committed_Abs_Tn_in_CO where
   "Committed_Abs_Tn_in_CO s k \<longleftrightarrow> (\<forall>n cl.
-    (\<exists>cts v rs deps. svr_state (svrs s k) (Tn (Tn_cl n cl)) = Commit cts v rs deps) \<or> 
+    (\<exists>cts v rs. svr_state (svrs s k) (Tn (Tn_cl n cl)) = Commit cts v rs) \<or> 
     ((\<exists>ts v. svr_state (svrs s k) (Tn (Tn_cl n cl)) = Prep ts v) \<and> 
-     (\<exists>cts kv_map deps. cl_state (cls s cl) = WtxnCommit cts kv_map deps \<and> cl_sn (cls s cl) = n)) \<longrightarrow>
+     (\<exists>cts kv_map. cl_state (cls s cl) = WtxnCommit cts kv_map \<and> cl_sn (cls s cl) = n)) \<longrightarrow>
     Tn (Tn_cl n cl) \<in> set (commit_order s k))"
 
 definition Committed_Abs_in_CO where
   "Committed_Abs_in_CO s k \<longleftrightarrow> (\<forall>t.
-    (\<exists>cts v rs deps. svr_state (svrs s k) t = Commit cts v rs deps) \<or> 
+    (\<exists>cts v rs. svr_state (svrs s k) t = Commit cts v rs) \<or> 
     ((\<exists>ts v. svr_state (svrs s k) t = Prep ts v) \<and>
-     (\<exists>cts kv_map deps. cl_state (cls s (get_cl_w t)) = WtxnCommit cts kv_map deps)) \<longrightarrow>
+     (\<exists>cts kv_map. cl_state (cls s (get_cl_w t)) = WtxnCommit cts kv_map)) \<longrightarrow>
     t \<in> set (commit_order s k))"
 
 definition CO_Sorted where
@@ -307,11 +301,11 @@ lemma kvs_of_s_init:
   "kvs_of_s (state_init) = (\<lambda>k. [\<lparr>v_value = undefined, v_writer = T0, v_readerset = {}\<rparr>])" oops
 
 abbreviation invariant_list_kvs where
-  "invariant_list_kvs s \<equiv> \<forall>k. CO_not_No_Ver s k \<and>  Fresh_wr_notin_rs s k"
+  "invariant_list_kvs s \<equiv> \<forall>k cl. CO_not_No_Ver s k \<and>  Fresh_wr_notin_rs s cl"
 
 abbreviation not_committing_ev where
-  "not_committing_ev e \<equiv> \<forall>cl kvt_map kv_map cts sn u. e \<noteq> RDone cl kvt_map sn u \<and>
-    e \<noteq> WCommit cl kv_map cts sn u"
+  "not_committing_ev e \<equiv> \<forall>cl kv_map cts sn u. e \<noteq> RDone cl kv_map sn u \<and>
+    e \<noteq> WCommit cl kv_map cts sn u"   
 
 lemma kvs_of_s_inv:
   assumes "state_trans s e s'"
@@ -323,16 +317,16 @@ lemma kvs_of_s_inv:
 subsection \<open>Transaction ID Freshness\<close>
 
 definition Sqn_Inv_nc where
-  "Sqn_Inv_nc s cl \<longleftrightarrow> (\<forall>cts kvm deps. cl_state (cls s cl) \<noteq> WtxnCommit cts kvm deps
-    \<longrightarrow> (\<forall>m \<in> get_sqns (kvs_of_s s) cl. m < cl_sn (cls s cl)))" (* commit events *)
+  "Sqn_Inv_nc s cl \<longleftrightarrow> (\<forall>cts kv_map. cl_state (cls s cl) \<noteq> WtxnCommit cts kv_map
+     \<longrightarrow> (\<forall>m \<in> get_sqns (kvs_of_s s) cl. m < cl_sn (cls s cl)))"
 
 definition Sqn_Inv_c where
-  "Sqn_Inv_c s cl \<longleftrightarrow> (\<forall>cts kvm deps. cl_state (cls s cl) = WtxnCommit cts kvm deps
-    \<longrightarrow> (\<forall>m \<in> get_sqns (kvs_of_s s) cl. m \<le> cl_sn (cls s cl)))"
+  "Sqn_Inv_c s cl \<longleftrightarrow> (\<forall>cts kv_map. cl_state (cls s cl) = WtxnCommit cts kv_map
+     \<longrightarrow> (\<forall>m \<in> get_sqns (kvs_of_s s) cl. m \<le> cl_sn (cls s cl)))"
 
 lemma t_is_fresh:
   assumes "Sqn_Inv_c s cl" and "Sqn_Inv_nc s cl"
-    and "cl_state (cls s cl) \<in> {WtxnPrep kv_map, RtxnInProg keys kvt_map}"
+    and "cl_state (cls s cl) \<in> {WtxnPrep kv_map, RtxnInProg keys kv_map}"
   shows "get_txn s cl \<in> next_txids (kvs_of_s s) cl" oops
 
 subsection \<open>committed At functions\<close>
@@ -351,20 +345,15 @@ lemma read_at_is_committed:
 
 
 subsection \<open>Kvt_map values of read_done\<close>
-definition Kvt_map_V_T where
-  "Kvt_map_V_T s cl \<longleftrightarrow> (\<forall>k t keys kvt_map v.
-    cl_state (cls s cl) = RtxnInProg keys kvt_map \<and> kvt_map k = Some (v, t) \<longrightarrow>
-     v = get_val (svr_state (svrs s k) t))"
-
 definition Rtxn_IdleK_notin_rs where
-  "Rtxn_IdleK_notin_rs s cl \<longleftrightarrow> (\<forall>k keys kvt_map t cts v rs deps.
-    cl_state (cls s cl) = RtxnInProg keys kvt_map \<and> k \<notin> keys \<and>
-    svr_state (svrs s k) t = Commit cts v rs deps \<longrightarrow> get_txn s cl \<notin> rs)"
+  "Rtxn_IdleK_notin_rs s cl \<longleftrightarrow> (\<forall>k keys kv_map t cts v rs.
+    cl_state (cls s cl) = RtxnInProg keys kv_map \<and> k \<notin> keys \<and>
+    svr_state (svrs s k) t = Commit cts v rs \<longrightarrow> get_txn s cl \<notin> rs)"
 
 definition Rtxn_RegK_Kvtm_Cmt_in_rs where
-  "Rtxn_RegK_Kvtm_Cmt_in_rs s cl \<longleftrightarrow> (\<forall>k keys kvt_map v t.
-    cl_state (cls s cl) = RtxnInProg keys kvt_map \<and> kvt_map k = Some (v, t) \<longrightarrow>
-    (\<exists>cts rs deps. svr_state (svrs s k) t = Commit cts v rs deps \<and> get_txn s cl \<in> rs))"
+  "Rtxn_RegK_Kvtm_Cmt_in_rs s cl \<longleftrightarrow> (\<forall>k keys kv_map v.
+    cl_state (cls s cl) = RtxnInProg keys kv_map \<and> kv_map k = Some v \<longrightarrow>
+    (\<exists>t cts rs. svr_state (svrs s k) t = Commit cts v rs \<and> get_txn s cl \<in> rs))"
 
 
 subsection \<open>Timestamp relations\<close>
@@ -372,8 +361,8 @@ subsection \<open>Timestamp relations\<close>
 definition Disjoint_RW where
   "Disjoint_RW s \<longleftrightarrow> ((\<Union>k. wtxns_dom (svr_state (svrs s k))) \<inter> Tn ` (\<Union>k. wtxns_rsran (svr_state (svrs s k))) = {})" (* not proven *)
 
-definition Disjoint_RW' where
-  "Disjoint_RW' s \<longleftrightarrow> (kvs_writers (kvs_of_s s) \<inter> Tn ` kvs_readers (kvs_of_s s) = {})" (* not proven *)
+(*definition Disjoint_RW' where
+  "Disjoint_RW' s \<longleftrightarrow> (kvs_writers (kvs_of_s s) \<inter> Tn ` kvs_readers (kvs_of_s s) = {})" (* not proven *)*)
 
 definition RO_has_rts where
   "RO_has_rts s \<longleftrightarrow> (\<forall>t. Tn t \<in> read_only_Txs (kvs_of_s s) \<longrightarrow> (\<exists>rts. rtxn_rts s t = Some rts))" (* not proven *)
@@ -433,95 +422,133 @@ lemma union_closed'_extend_rel:
 
 
 lemma visTx'_new_writer: "kvs_writers K' = insert t (kvs_writers K) \<Longrightarrow>
-  snd ` t_wr_deps = {t} \<Longrightarrow> visTx' K' (u \<union> t_wr_deps) = insert t (visTx' K u)"
-  by (auto simp add: visTx'_def)
+  visTx' K' (insert t u) = insert t (visTx' K u)" oops
 
 lemma insert_wr_t_closed':
   assumes "closed' K u r"
     and "closed_general {t} (r\<inverse>) (visTx' K u \<union> read_only_Txs K)"
     and "read_only_Txs K' = read_only_Txs K"
     and "kvs_writers K' = insert t (kvs_writers K)"
-    and "snd ` t_wr_deps = {t}"
-  shows "closed' K' (u \<union> t_wr_deps) r"
-  using assms
-  by (auto simp add: closed'_def visTx'_new_writer intro: closed_general_set_union_closed)
+  shows "closed' K' (insert t u) r" oops
 
 \<comment> \<open>insert (k, t) in version's deps - used in get_ctx\<close>
 lemma visTx'_observes_t:
-  "t \<in> kvs_writers K \<Longrightarrow> visTx' K (insert (k, t) deps) = insert t (visTx' K deps)"
-  by (simp add: visTx'_def)
+  "t \<in> kvs_writers K \<Longrightarrow> visTx' K (insert t deps) = insert t (visTx' K deps)" oops
 
 lemma insert_kt_to_deps_closed':
   assumes "closed' K deps r"
     and "t \<in> kvs_writers K"
     and "closed_general {t} (r\<inverse>) (visTx' K deps \<union> read_only_Txs K)"
-  shows "closed' K (insert (k, t) deps) r"
-  using assms
-  by (auto simp add: closed'_def visTx'_observes_t intro: closed_general_set_union_closed)
+  shows "closed' K (insert t deps) r" oops
 
 
 \<comment> \<open>concrete read_done closedness\<close>
 
 \<comment> \<open>premises\<close>
-lemma get_ctx_reformulate:
-  assumes "cl_state (cls s cl) = RtxnInProg keys kvt_map"
-    and "Kvt_map_t_Committed s cl"
-  shows "get_ctx s kvt_map = (\<Union>k\<in>dom kvt_map. (let t = snd (the (kvt_map k)) in 
-    insert (k, t) (get_dep_set (svr_state (svrs s k) t))))" oops
   
 lemma get_ctx_closed:
-  assumes "\<And>k. k \<in> dom kvt_map \<Longrightarrow> let t = snd (the (kvt_map k)) in
-      closed' K (insert (k, t) (get_dep_set (svr_state (svrs s k) t))) r"
-    and "cl_state (cls s cl) = RtxnInProg keys kvt_map"
-    and "Kvt_map_t_Committed s cl"
-    and "Finite_Dom_Kvt_map s cl"
-  shows "closed' K (get_ctx s kvt_map) r" oops
+  assumes "\<And>k. k \<in> dom kv_map \<Longrightarrow>
+      let t = read_at (svr_state (svrs s k)) (gst (cls s cl)) cl in
+      closed' K (insert t (get_dep_set (svr_state (svrs s k) t))) r"
+    and "cl_state (cls s cl) = RtxnInProg (dom kv_map) kv_map"
+    and "Rtxn_RegK_Kvtm_Cmt_in_rs s cl"
+    and "Finite_Dom_Kv_map_rd s cl"
+  shows "closed' K (get_ctx s cl (dom kv_map)) r" oops
+
+lemma v_writer_kvs_of_s:
+  assumes "\<forall>k. CO_not_No_Ver s k"
+  shows "v_writer ` (\<lambda>t. case svr_state (svrs s k) t of
+      Prep ts v \<Rightarrow> \<lparr>v_value = v, v_writer = t, v_readerset = {}\<rparr>
+    | Commit cts v rs \<Rightarrow> \<lparr>v_value = v, v_writer = t,
+        v_readerset = {t \<in> rs. get_sn t < cl_sn (cls s (get_cl t))}\<rparr>) ` set (commit_order s k) =
+   {t \<in> set (commit_order s k). \<exists>ts v cts rs deps.
+        svr_state (svrs s k) t \<in> {Prep ts v, Commit cts v rs}}" oops
+
+lemma v_readerset_kvs_of_s_k:
+  assumes "\<forall>k. CO_not_No_Ver s k"
+    and "t_wr \<in> set (commit_order s k)"
+  shows "v_readerset (case svr_state (svrs s k) t_wr of
+      Prep ts v \<Rightarrow> \<lparr>v_value = v, v_writer = t_wr, v_readerset = {}\<rparr>
+    | Commit cts v rs \<Rightarrow> \<lparr>v_value = v, v_writer = t_wr,
+        v_readerset = {t \<in> rs. get_sn t < cl_sn (cls s (get_cl t))}\<rparr>) = 
+   {t. \<exists>cts v rs. svr_state (svrs s k) t_wr = Commit cts v rs \<and>
+      t \<in> rs \<and> get_sn t < cl_sn (cls s (get_cl t))}" oops
+
+lemma v_readerset_kvs_of_s:
+  assumes "\<forall>k. CO_not_No_Ver s k"
+  shows "(\<Union>k. \<Union>t_wr\<in>set (commit_order s k). v_readerset (case svr_state (svrs s k) t_wr of
+      Prep ts v \<Rightarrow> \<lparr>v_value = v, v_writer = t_wr, v_readerset = {}\<rparr>
+    | Commit cts v rs \<Rightarrow> \<lparr>v_value = v, v_writer = t_wr,
+        v_readerset = {t \<in> rs. get_sn t < cl_sn (cls s (get_cl t))}\<rparr>)) = 
+   {t. \<exists>k. \<exists>t_wr \<in> set (commit_order s k).
+      \<exists>cts v rs. svr_state (svrs s k) t_wr = Commit cts v rs \<and>
+      t \<in> rs \<and> get_sn t < cl_sn (cls s (get_cl t))}" oops
 
 lemma read_done_same_writers:
-  assumes "read_done cl kvt_map sn u'' s s'"
+  assumes "read_done cl kv_map sn u'' s s'"
     and "\<forall>k. CO_not_No_Ver s k"
     and "\<forall>k. CO_not_No_Ver s' k"
   shows "kvs_writers (kvs_of_s s') = kvs_writers (kvs_of_s s)" oops
 
 lemma read_done_new_read:
-  assumes "read_done cl kvt_map sn u'' s s'"
+  assumes "read_done cl kv_map sn u'' s s'"
     and "\<forall>k. CO_not_No_Ver s k"
     and "\<forall>k. CO_not_No_Ver s' k"
     and "\<forall>k. Committed_Abs_in_CO s k"
     and "\<forall>k. T0_in_CO s k"
-    and "Finite_Dom_Kvt_map s cl"
-    and "Kvt_map_t_Committed s cl"
-    and "Rtxn_RegK_in_rs s cl"
+    and "Finite_Dom_Kv_map_rd s cl"
+    and "Rtxn_RegK_Kvtm_Cmt_in_rs s cl"
+    and "Rtxn_RegK_Kvtm_Cmt_in_rs s cl"
     and "Tn (get_txn s cl) \<notin> kvs_writers (kvs_of_s s)"
   shows "read_only_Txs (kvs_of_s s') = insert (Tn (get_txn s cl)) (read_only_Txs (kvs_of_s s))" oops
 
 lemma read_done_WR_onK:
-  assumes "read_done cl kvt_map sn u'' s s'"
-  shows "R_onK WR (kvs_of_s s') = (\<Union>y\<in>snd ` ran kvt_map. {(y, Tn (get_txn s cl))}) \<union> R_onK WR (kvs_of_s s)" oops
+  assumes "read_done cl kv_map sn u'' s s'"
+  shows "R_onK WR (kvs_of_s s') = (\<Union>y\<in>snd ` ran kv_map. {(y, Tn (get_txn s cl))}) \<union> R_onK WR (kvs_of_s s)" oops
 (* not proven *)
 
 lemma read_done_extend_rel:
-  assumes "read_done cl kvt_map sn u'' s s'"
-  shows "R_CC (kvs_of_s s') = (\<Union>y\<in>snd ` ran kvt_map. {(y, Tn (get_txn s cl))}) \<union> R_CC (kvs_of_s s)" oops
+  assumes "read_done cl kv_map sn u'' s s'"
+  shows "R_CC (kvs_of_s s') = (\<Union>y\<in>snd ` ran kv_map. {(y, Tn (get_txn s cl))}) \<union> R_CC (kvs_of_s s)" oops
 
 \<comment> \<open>read_done closedness (canCommit)\<close>
 lemma read_done_ctx_closed:
   assumes "closed' (kvs_of_s s) (cl_ctx (cls s cl)) (R_CC (kvs_of_s s))"
-    and "closed' (kvs_of_s s) (get_ctx s kvt_map) (R_CC (kvs_of_s s))"
+    and "closed' (kvs_of_s s) (get_ctx s cl keys) (R_CC (kvs_of_s s))"
     and "kvs_writers (kvs_of_s s') = kvs_writers (kvs_of_s s)"
     and "read_only_Txs (kvs_of_s s') = insert (Tn (get_txn s cl)) (read_only_Txs (kvs_of_s s))"
-    and "Tn (get_txn s cl) \<notin> ((R_CC (kvs_of_s s))\<inverse>)\<^sup>* `` (visTx' (kvs_of_s s) (cl_ctx (cls s cl) \<union> get_ctx s kvt_map))"
-    and "R_CC (kvs_of_s s') = (\<Union>y\<in>snd ` ran kvt_map. {(y, Tn (get_txn s cl))}) \<union> R_CC (kvs_of_s s)"
+    and "Tn (get_txn s cl) \<notin> ((R_CC (kvs_of_s s))\<inverse>)\<^sup>* ``
+      (visTx' (kvs_of_s s) (cl_ctx (cls s cl) \<union> get_ctx s cl keys))"
+    and "R_CC (kvs_of_s s') = (\<Union>y\<in>snd ` ran kv_map. {(y, Tn (get_txn s cl))}) \<union> R_CC (kvs_of_s s)"
     and "Finite_t_Ran_Kvt_map s cl"
-    and "cl_state (cls s cl) = RtxnInProg keys kvt_map"
-  shows "closed' (kvs_of_s s') (cl_ctx (cls s cl) \<union> get_ctx s kvt_map) (R_CC (kvs_of_s s'))" oops                        
+    and "cl_state (cls s cl) = RtxnInProg keys kv_map"
+  shows "closed' (kvs_of_s s') (cl_ctx (cls s cl) \<union> get_ctx s cl keys) (R_CC (kvs_of_s s'))" oops
+
+\<comment> \<open>write_commit closedness (canCommit)\<close>
+lemma write_commit_WR_onK:
+  assumes "write_commit cl kv_map commit_t sn u'' s s'"
+  shows "R_onK WR (kvs_of_s s') = R_onK WR (kvs_of_s s)" oops (* not proven *)
+
+lemma write_commit_same_rel:
+  assumes "write_commit cl kv_map commit_t sn u'' s s'"
+  shows "R_CC (kvs_of_s s') = R_CC (kvs_of_s s)" oops
+
+lemma write_commit_ctx_closed:
+  assumes "write_commit cl kv_map commit_t sn u'' s s'"
+    and "closed' (kvs_of_s s) (cl_ctx (cls s cl)) (R_CC (kvs_of_s s))"
+    and "closed_general {get_wtxn s cl} ((R_CC (kvs_of_s s))\<inverse>)
+          (visTx' (kvs_of_s s) (cl_ctx (cls s cl)) \<union> read_only_Txs (kvs_of_s s))"
+    and "read_only_Txs (kvs_of_s s') = read_only_Txs (kvs_of_s s)"
+    and "kvs_writers (kvs_of_s s') = insert (get_wtxn s cl) (kvs_writers (kvs_of_s s))"
+  shows "closed' (kvs_of_s s') (insert (get_wtxn s cl) (cl_ctx (cls s cl))) (R_CC (kvs_of_s s'))"
+  oops (* not proven *)
 
 
 subsection \<open>CanCommit\<close>
 
-lemmas canCommit_defs = ET_CC.canCommit_def R_CC_def R_onK_def
+lemma the_T0: "(THE i. i = 0 \<and> [T0] ! i = T0) = 0" oops
 
-lemma the_T0: "(THE i. i = 0 \<and> [T0] ! i = T0) = 0" by auto
+lemmas canCommit_defs = ET_CC.canCommit_def R_CC_def R_onK_def
 
 lemma visTx_visTx': "\<comment> \<open>\<forall>k t. (k, t) \<in> u \<longrightarrow> t \<in> set (commit_order s k) \<Longrightarrow>\<close>
   visTx (kvs_of_s s) (view_of (commit_order s) u) = visTx' (kvs_of_s s) u" oops (* not proven *)
@@ -529,49 +556,17 @@ lemma visTx_visTx': "\<comment> \<open>\<forall>k t. (k, t) \<in> u \<longrighta
 lemma closed_closed': "\<comment> \<open>\<forall>k t. (k, t) \<in> u \<longrightarrow> t \<in> set (commit_order s k) \<Longrightarrow>\<close>
   closed (kvs_of_s s) (view_of (commit_order s) u) r = closed' (kvs_of_s s) u r" oops
 
-lemma visTx'_subset_writers:
-  "visTx' (kvs_of_s s) (get_view s cl) \<subseteq> kvs_writers (kvs_of_s s)" oops
-
 lemma visTx'_cl_ctx_subset_writers:
   "visTx' (kvs_of_s s) (cl_ctx (cls s cl)) \<subseteq> kvs_writers (kvs_of_s s)" oops
 
-lemma visTx'_deps_subset_writers: 
-  "svr_state (svrs s k) t = Commit cts v rs deps
-    \<Longrightarrow> visTx' (kvs_of_s s) deps \<subseteq> kvs_writers (kvs_of_s s)" oops
-
-lemma visTx'_cl_deps_subset_writers: 
-  "cl_state (cls s cl) = WtxnCommit cts kvm deps
-    \<Longrightarrow> visTx' (kvs_of_s s) deps \<subseteq> kvs_writers (kvs_of_s s)" oops
+lemma visTx'_wtxn_deps_subset_writers: 
+  "wtxn_deps s t = deps \<Longrightarrow> visTx' (kvs_of_s s) deps \<subseteq> kvs_writers (kvs_of_s s)" oops
 
 lemma "kvs_writers (kvs_of_s s) \<subseteq> (\<Union>k. wtxns_dom (svr_state (svrs s k)))"(* not proven *)
   oops
 
 lemma "kvs_readers (kvs_of_s s) \<subseteq> (\<Union>k. wtxns_rsran (svr_state (svrs s k)))"(* not proven *)
   oops
-
-definition closed_general :: "'v set \<Rightarrow> 'v rel \<Rightarrow> 'v set \<Rightarrow> bool" where
-  "closed_general vis r r_only \<equiv> vis = ((r^*) `` (vis)) - r_only"
-
-lemma closed'_generalize: "closed' K u r = closed_general (visTx' K u) (r^-1) (read_only_Txs K)" oops
-
-lemma union_closed_general:
-  "closed_general vis r r_only \<Longrightarrow> closed_general vis' r r_only
-    \<Longrightarrow> closed_general (vis \<union> vis') r r_only" oops
-
-lemma visTx_union_distr: "visTx' K (u \<union> u') = visTx' K u \<union> visTx' K u'" oops
-
-lemma union_closed: "closed' K u r \<Longrightarrow> closed' K u' r \<Longrightarrow> closed' K (u \<union> u') r" oops
-
-lemma visTx'_insert:
-  "snd t \<in> kvs_writers K \<Longrightarrow> visTx' K (insert t u) = insert (snd t) (visTx' K u)" oops
-
-lemma insert_t_closed_general:
-  "t \<notin> vis \<Longrightarrow> t \<notin> r_only \<Longrightarrow> (\<And>x. (t, x) \<in> r^* \<Longrightarrow> x \<in> vis \<or> x \<in> r_only \<or> x = t)
-    \<Longrightarrow> closed_general vis r r_only \<Longrightarrow> closed_general (insert t vis) r r_only" oops
-
-lemma insert_t_closed:
-  "get_wtxn s cl \<in> kvs_writers K \<Longrightarrow> closed' K (cl_ctx (cls s cl)) r \<Longrightarrow>
-    closed' K (insert (k, get_wtxn s cl) (cl_ctx (cls s cl))) r" oops (* not proven *)
 
 definition RO_le_gst :: "'v global_conf \<Rightarrow> cl_id \<Rightarrow> txid set" where
   "RO_le_gst s cl \<equiv> {t \<in> read_only_Txs (kvs_of_s s). \<exists>t'. t = Tn t' \<and> the (rtxn_rts s t') \<le> gst (cls s cl)}"
@@ -583,47 +578,35 @@ definition RO_WO_Inv where
 subsection \<open>Ctx Invariants\<close>
 
 definition View_Init where
-  "View_Init s cl \<longleftrightarrow> (\<forall>k. (k, T0) \<in> cl_ctx (cls s cl))"
+  "View_Init s cl \<longleftrightarrow> (T0 \<in> cl_ctx (cls s cl))"
 
-\<comment> \<open>deps are committed\<close>
+\<comment> \<open>deps are committed\<close> (* broken : not proven *)
 definition Ctx_Committed where
-  "Ctx_Committed s \<longleftrightarrow> (\<forall>cl k t. (k, t) \<in> cl_ctx (cls s cl) \<longrightarrow>
-    is_committed (svr_state (svrs s k) t) \<or> 
-    (\<exists>cts kvm deps. cl_state (cls s cl) = WtxnCommit cts kvm deps \<and>
-      k \<in> dom kvm \<and> t = get_wtxn s cl))"
+  "Ctx_Committed s \<longleftrightarrow> (\<forall>cl t k. t \<in> cl_ctx (cls s cl) \<and> t \<in> set (commit_order s k)  \<longrightarrow>
+    (is_committed (svr_state (svrs s k) t) \<or> 
+    (\<exists>cts kv_map. cl_state (cls s cl) = WtxnCommit cts kv_map \<and> k \<in> dom kv_map \<and> t = get_wtxn s cl)))"
 
-definition Deps_Committed where
-  "Deps_Committed s \<longleftrightarrow> (\<forall>k t k' t' cts v rs deps. svr_state (svrs s k) t = Commit cts v rs deps \<and>
-    (k', t') \<in> deps \<longrightarrow> is_committed (svr_state (svrs s k') t'))"
+definition Wtxn_Deps_Committed where
+  "Wtxn_Deps_Committed s \<longleftrightarrow> (\<forall>t k t' deps. wtxn_deps s t' = deps \<and>
+    t \<in> deps \<and> t \<in> set (commit_order s k) \<longrightarrow> is_committed (svr_state (svrs s k) t))"
 
-definition Cl_Deps_Committed where
-  "Cl_Deps_Committed s \<longleftrightarrow> (\<forall>cl k t cts kv_map deps. cl_state (cls s cl) = WtxnCommit cts kv_map deps \<and>
-    (k, t) \<in> deps \<longrightarrow> is_committed (svr_state (svrs s k) t))"
-
-definition Cl_Ctx_Sub_CO where
-  "Cl_Ctx_Sub_CO s k \<longleftrightarrow> (\<forall>cl t. (k, t) \<in> cl_ctx (cls s cl) \<longrightarrow> t \<in> set (commit_order s k))"
-
-definition Get_Ctx_Sub_CO where
-  "Get_Ctx_Sub_CO s k \<longleftrightarrow> (\<forall>cl t keys kvt_map. cl_state (cls s cl) = RtxnInProg keys kvt_map \<and>
-    (k, t) \<in> get_ctx s kvt_map \<longrightarrow> t \<in> set (commit_order s k))"
+definition Get_Ctx_Commited where
+  "Get_Ctx_Commited s k \<longleftrightarrow> (\<forall>cl t keys kv_map. cl_state (cls s cl) = RtxnInProg keys kv_map \<and>
+    t \<in> get_ctx s cl keys \<and> t \<in> set (commit_order s k) \<longrightarrow> is_committed (svr_state (svrs s k) t))"
 
 definition Deps_Closed where
   "Deps_Closed s cl \<longleftrightarrow> (closed' (kvs_of_s s) (cl_ctx (cls s cl)) (R_CC (kvs_of_s s)) \<and> 
-    (\<forall>k t cts v rs kv_map deps. svr_state (svrs s k) t = Commit cts v rs deps \<or>
-      cl_state (cls s cl) = WtxnCommit cts kv_map deps \<longrightarrow>
+    (\<forall>k t cts v rs kv_map deps. svr_state (svrs s k) t = Commit cts v rs \<or>
+      cl_state (cls s cl) = WtxnCommit cts kv_map \<longrightarrow>
       closed' (kvs_of_s s) deps (R_CC (kvs_of_s s))))" (* not proven *)
 
 
 subsection \<open>View Shift\<close>
 
-lemma get_view_grows:
-  assumes "state_trans s e s'" and "Gst_le_Min_Lst_map s cl"
-  shows "(\<lambda>k. get_view s cl `` {k}) \<sqsubseteq> (\<lambda>k. get_view s' cl `` {k})" oops
-
 definition Cl_Ctx_WtxnCommit where
   "Cl_Ctx_WtxnCommit s cl \<longleftrightarrow>
-    (\<forall>cts kv_map deps k. cl_state (cls s cl) = WtxnCommit cts kv_map deps \<and> k \<in> dom kv_map \<longrightarrow>
-      (k, get_wtxn s cl) \<in> cl_ctx (cls s cl))"
+    (\<forall>cts kv_map. cl_state (cls s cl) = WtxnCommit cts kv_map \<longrightarrow>
+      get_wtxn s cl \<in> cl_ctx (cls s cl))"
 
 lemma read_commit_added_txid:
   assumes "read_done cl kv_map sn u s s'"
@@ -636,19 +619,19 @@ subsection \<open>Fp Property\<close>
 \<comment> \<open>Fingerprint content invariant and Lemmas for proving the fp_property\<close>
 
 definition RegR_Fp_Inv where
-  "RegR_Fp_Inv s k \<longleftrightarrow> (\<forall>t keys kv_map cts v rs deps.
+  "RegR_Fp_Inv s k \<longleftrightarrow> (\<forall>t keys kv_map cts v rs.
     cl_state (cls s (get_cl t)) = RtxnInProg keys kv_map \<and> k \<in> keys \<and> kv_map k = None \<and>
     svr_state (svrs s k) (read_at (svr_state (svrs s k)) (gst (cls s (get_cl t))) (get_cl t))
-       = Commit cts v rs deps \<longrightarrow>
-    v = v_value (last_version (kvs_of_s s k)
-      (view_of (commit_order s) (get_view s (get_cl t)) k)))"
+       = Commit cts v rs \<longrightarrow>
+    v = v_value ((kvs_of_s s k) !
+      Max (view_of (commit_order s) (cl_ctx (cls s (get_cl t)) \<union> get_ctx s (get_cl t) keys) k)))"
  (* not proven *)
 
 definition Rtxn_Fp_Inv where
-  "Rtxn_Fp_Inv s cl \<longleftrightarrow> (\<forall>k t keys kvt_map v.
-    cl_state (cls s cl) = RtxnInProg keys kvt_map \<and> kvt_map k = Some (v, t) \<longrightarrow>
-     v = v_value (last_version (kvs_of_s s k)
-      (view_of (commit_order s) (cl_ctx (cls s cl) \<union> get_ctx s kvt_map) k)))"
+  "Rtxn_Fp_Inv s cl \<longleftrightarrow> (\<forall>k keys kv_map v.
+    cl_state (cls s cl) = RtxnInProg keys kv_map \<and> kv_map k = Some v \<longrightarrow>
+     v = v_value ((kvs_of_s s k) !
+        Max (view_of (commit_order s) (cl_ctx (cls s cl) \<union> get_ctx s cl keys) k)))"
 (* not proven *)
 
 subsection\<open>Proofs in progress\<close>
@@ -687,8 +670,7 @@ lemma view_of_ext_corder_cl_ctx:
   assumes "\<And>k. distinct (ext_corder (get_wtxn gs cl) kv_map (commit_order gs) k)"
   shows "view_of (commit_order gs) (cl_ctx (cls gs cl)) \<sqsubseteq> 
          view_of (ext_corder (get_wtxn gs cl) kv_map (commit_order gs)) 
-                 (cl_ctx (cls gs cl) \<union> dom kv_map \<times> {get_wtxn gs cl})" oops
-
+                 (insert (get_wtxn gs cl) (cl_ctx (cls gs cl)))" oops
 
 \<comment> \<open>more lemmas about view updates\<close>
 lemma view_of_update:
@@ -696,7 +678,7 @@ lemma view_of_update:
     "i = length (cord k)"  
     "cord' k = cord k @ [t]"
     "t \<notin> set (cord k)"
-    "(k, t) \<in> deps"
+    "t \<in> deps"
   shows "i \<in> view_of cord' deps k" oops
 
 \<comment> \<open>lemmas related to commit order (CO)\<close>
@@ -757,7 +739,7 @@ lemma write_commit_views_of_s:
   assumes "write_commit cl kv_map commit_t sn u'' s s'"
   shows "views_of_s s' = 
          (\<lambda>cl'. view_of (ext_corder (get_wtxn s cl) kv_map (commit_order s))    
-                        (if cl' = cl then cl_ctx (cls s cl) \<union> dom kv_map \<times> {get_wtxn s cl} 
+                        (if cl' = cl then insert (get_wtxn s cl) (cl_ctx (cls s cl)) 
                          else cl_ctx (cls s cl')))" oops
 
 lemma full_view_elem: "i \<in> full_view vl \<longleftrightarrow> i < length vl" oops
@@ -768,23 +750,22 @@ lemma length_update_kv_bound:
 
 subsubsection \<open>View Wellformedness\<close>
 
-\<comment> \<open>NOT USED
-lemma v_writer_set_commit_order_eq:
-  assumes "CO_not_No_Ver s k"                   
-  shows "v_writer ` set (kvs_of_s s k) = set (commit_order s k)"\<close>
-
+definition FTid_notin_Ctx where
+  "FTid_notin_Ctx s cl \<longleftrightarrow> (\<forall>n cl'. (n > cl_sn (cls s cl) \<longrightarrow> Tn (Tn_cl n cl) \<notin> cl_ctx (cls s cl')) \<and>
+    (cl' \<noteq> cl \<longrightarrow> get_wtxn s cl \<notin> cl_ctx (cls s cl')))"
 
 lemma write_commit_views_of_s_other_cl_inv:
   assumes "write_commit cl kv_map cts sn u s s'"
     and "\<And>k. CO_Distinct s' k"
-    and "\<And>k. Cl_Ctx_Sub_CO s k"
+    and "FTid_notin_Ctx s cl"
     and "cl' \<noteq> cl"
   shows "views_of_s s' cl' = views_of_s s cl'" oops
 
 lemma reach_kvs_expands [simp]:
-  assumes "state_trans s e s'" and "\<And>cl. Sqn_Inv_c s cl" and "\<And>cl. Sqn_Inv_nc s cl"
-    and "\<And>cl. PTid_Inv s cl" and "\<And>cl. FTid_Wtxn_Inv s cl"
-    and "Kvs_Not_Emp s" and "invariant_list_kvs s"
+  assumes "state_trans s e s'"
+    and "\<And>cl. Sqn_Inv_c s cl"
+    and "\<And>cl. Sqn_Inv_nc s cl"
+    and "invariant_list_kvs s"
   shows "kvs_of_s s \<sqsubseteq>\<^sub>k\<^sub>v\<^sub>s kvs_of_s s'" oops
 
 definition Views_of_s_Wellformed where
@@ -792,8 +773,9 @@ definition Views_of_s_Wellformed where
 
 
 subsection \<open>Refinement Proof\<close>
-abbreviation invariant_list where
+definition invariant_list where
   "invariant_list s \<equiv> (\<forall>cl k. invariant_list_kvs s \<and> Sqn_Inv_c s cl \<and> Sqn_Inv_nc s cl
-    \<and> Views_of_s_Wellformed s cl \<and> Rtxn_Fp_Inv s cl \<and> CO_Distinct s k \<and> Ctx_Committed s)"
+    \<and> Deps_Closed s cl \<and> Views_of_s_Wellformed s cl \<and> Rtxn_Fp_Inv s cl \<and> CO_Distinct s k
+    \<and> T0_in_CO s k \<and> T0_First_in_CO s k \<and> View_Init s cl \<and> FTid_notin_Ctx s cl)"
 
 end
